code/ecdsap256/Hacl.Impl.P.LowLevel.fsti
@@ -317,7 +317,7 @@ val shift1: #c: curve -> t: widefelem c -> t1: widefelem c -> Stack unit
 inline_for_extraction noextract 
 val upload_one_montg_form: #c: curve -> b: felem c -> Stack unit
   (requires fun h -> live h b)
-  (ensures fun h0 _ h1 -> modifies (loc b) h0 h1 )
+  (ensures fun h0 _ h1 -> modifies (loc b) h0 h1 /\ as_nat c h1 b = toDomain_ #c 1)
 
 
 inline_for_extraction noextract
